pure/Learn.Universe.fst
@@ -1,0 +1,47 @@
+module Learn.Universe
+
+irreducible let __universe__ : unit = ()
+
+/// Redefining [FStar.Universe] in order to expose their definitions for normalisation.
+
+type raise_t ([@@@ strictly_positive] a : Type u#a) : Type u#(max a b)
+  = | RaiseVal of a
+
+[@@ __universe__]
+let raise_val (#a : Type u#a) (x : a) : raise_t u#a u#b a
+  = RaiseVal x
+
+[@@ __universe__]
+let downgrade_val (#a : Type u#a) (y : raise_t u#a u#b a) : a
+  = let RaiseVal x = y in x
+
+
+(***** arrow *)
+
+[@@ __universe__]
+let lift_dom #a (#b : a -> Type u#c) (q : (x : a) -> b x) : (x : raise_t u#a u#b a) -> (b (downgrade_val x)) =
+  fun v -> q (downgrade_val v)
+
+[@@ __universe__]
+let lift_codom (#a : Type u#c) (#b : a -> Type) (q: (x : a) -> b x) : (x : a) -> raise_t u#a u#b (b x) =
+  fun v -> raise_val (q v)
+
+
+(***** PURE *)
+
+[@@ __universe__]
+let raise_pure_wp' (#a : Type u#a) (wp : pure_wp' a) : pure_wp' (raise_t u#a u#b a)
+  = fun pt -> wp (fun x -> pt (raise_val u#a u#b x))
+
+[@@ __universe__]
+let raise_pure_wp (#a : Type u#a) (wp : pure_wp a) : pure_wp (raise_t u#a u#b a)
+  =
+    FStar.Monotonic.Pure.elim_pure_wp_monotonicity wp;
+    FStar.Monotonic.Pure.as_pure_wp (raise_pure_wp' #a wp)
+
+inline_for_extraction
+let raise_pure_val (#a : Type u#a) (wp : pure_wp a) (f : unit -> PURE a wp)
+  : unit -> PURE (raise_t u#a u#b a) (raise_pure_wp u#a u#b wp)
+  =
+    FStar.Monotonic.Pure.elim_pure_wp_monotonicity wp;
+    fun () -> raise_val u#a u#b (f ())
